Bad Hoare triple on monad

Test.v
@@ -1,4 +1,4 @@
-Require Import Program.
+Require Import Program Arith.
 
 Set Implicit Arguments.
 
@@ -24,7 +24,7 @@ Definition state_bind A (st_a : State A) B  (f : A -> State B) :=
   fun  s => let (a,s) := st_a s in
             f a s.
 
-Definition put (x : S) : State unit :=
+Definition put (x : S) : State () :=
   fun _ => (tt,x).
 
 Definition get : State S :=
@@ -40,21 +40,31 @@ Notation "'perf' x '<-' m ';' e" := (state_bind m (fun x => e))
 
 Open Scope monad_scope.
 
-Definition hoareTripleS {A} (P : S -> Prop) (m : State A) (Q : A -> S -> Prop) : Prop :=
+Definition Assertion := S -> Prop.
+
+Definition hoareTripleS {A} (P : Assertion) (m : State A) (Q : A -> Assertion) : Prop :=
   forall (s : S), P s -> let (a, s') := m s in Q a s'.
 
 Notation "{{ P }} m {{ Q }}" := (hoareTripleS P m Q)
   (at level 90, format "'[' '[' {{  P  }}  ']' '/  ' '[' m ']' '['  {{  Q  }} ']' ']'") : monad_scope.
 
-Lemma conjProp (A : Type ) (P R : S -> Prop) (Q : A -> S -> Prop) m :
-  {{ P }} m {{ Q}} -> {{R}} m {{fun _ => R}} -> {{fun s => P s/\ R s}} m {{fun a s => Q a s/\ R s}}.
-  Proof.
-  intros H1 H2 s [H3 H4].
-  apply H1 in H3.
-  apply H2 in H4.
-  destruct (m s).
-  tauto.
-  Qed.
+Lemma ret  (A : Type) (a : A) (P : A -> Assertion) : {{ P a }} state_pure a {{ P }}.
+Proof.
+intros s H; trivial.
+Qed.
+
+(* Triplet de hoare sur la séquence *)
+Lemma bind  (A B : Type) (m : State A) (f : A -> State B) (P : Assertion)( Q : A -> Assertion) (R : B -> Assertion) :
+  (forall a, {{ Q a }} f a {{ R }}) -> {{ P }} m {{ Q }} -> {{ P }} perf x <- m ; f x {{ R }}.
+Proof. 
+intros H1 H2 s H3.
+unfold state_bind.
+case_eq (m s).
+intros.
+apply H2 in H3.
+case_eq (f a s0).
+intros b s'' H5.
+Admitted.
 
 Definition wp {A : Type} (P : A -> S -> Prop) (m : State A) :=
   fun s => let (a,s') := m s in P a s'.
@@ -85,9 +95,24 @@ Lemma assoc (A B C : Type)(m : State A)(f : A -> State B)(g : B -> State C) :
   extensionality s; unfold state_bind; case (m s); trivial; tauto.
   Qed.
 
-
-Definition modify (f : S -> S) : State unit :=
+Definition modify (f : S -> S) : State () :=
   perf s <- get ; put (f s).
+
+Lemma l_put (s : S) (P : unit -> Assertion) : {{ fun _ => P tt s }} put s {{ P }}.
+Proof.
+intros s0 H;trivial.
+Qed.
+
+Lemma l_get (P : S -> Assertion) : {{ fun s => P s s }} get {{ P }}.
+Proof.
+intros s H; trivial.
+Qed.
+
+Lemma bindRev (A B : Type) (m : State A) (f : A -> State B) (P : Assertion)( Q : A -> Assertion) (R : B -> Assertion) :
+  {{ P }} m {{ Q }} -> (forall a, {{ Q a }} f a {{ R }}) -> {{ P }} perf x <- m ; f x {{ R }}.
+Proof.
+intros; eapply bind ; eassumption.
+Qed.
 
 (* End state_monad.
 
@@ -95,18 +120,19 @@ Section loop_monad. *)
 
 Definition LoopT a : Type := (forall (r : Type), (a -> State r) -> State r).
 
-Definition runLoopT {a r} (loop : LoopT a) : (a -> State r) -> State r :=
-  fun next => loop r next.
+Definition runLoopT {a r} (loop : LoopT a) (next : a -> State r) :  State r :=
+  loop r next.
+(* next : (a -> LoopT r) *)
 
 (* Arguments runLoopT {_} {_} {_} {_}. *)
 
 Definition loopT_pure {A} (a : A) : LoopT A :=
-  fun _ cont => cont a.
+  fun _ next => next a.
 
 (* >>= for Loop *)
 Definition loopT_bind {A} (x : LoopT A) {B} (k : A -> LoopT B) : LoopT B :=
-  (fun _ cont =>
-    let f' := (fun a => runLoopT (k a) cont) in
+  (fun _ next =>
+    let f' := (fun a => runLoopT (k a) next) in
     runLoopT x f').
 
 (* Variable m : Type -> Type. *)
@@ -122,7 +148,7 @@ Definition loopT_liftT {A} (x : State A) : LoopT A :=
 Definition stepLoopT {e a}  (body : LoopT e (State S) a) (next : a -> (State S) e) : (State S) e :=
   runLoopT body (return_) next. *)
 
-Definition stepLoopT {a} (body : LoopT a) (next : a -> State unit) : State unit :=
+Definition stepLoopT {a} (body : LoopT a) (next : a -> State ()) : State () :=
   runLoopT body next.
 
 (* exit = 
@@ -130,25 +156,40 @@ fun (m : Type -> Type) (a : Type) (_ : Monad m) (r : Type) (fin : () -> m r)
   (_ : a -> m r) => fin tt
      : forall (m : Type -> Type) (a : Type), Monad m -> LoopT () m a *)
 (* 
-Definition exit {a}: LoopT unit a :=
+Definition exit {a}: LoopT () a :=
   fun _ fin _ => fin tt. *)
 
 Import List.
 
-Definition foreach''{a} (values : list a) {c} (body : a -> LoopT c) : State unit :=
+Definition foreach''{v} (values : list v) {a} (body : v -> LoopT a) : State () :=
   fold_right
     (fun x next => stepLoopT (body x) (fun _ => next))
     (state_pure tt)
     values.
 
-Definition foreach'(min max : nat) {a} (body : nat -> LoopT a) : State unit :=
+Definition foreach'(min max : nat) (body : nat -> LoopT ()) : State () :=
   foreach'' (seq min (max-min)) body.
 
 Notation "'for' i '=' min 'to' max '{{' body }}" := (foreach' min max (fun i => (loopT_liftT body))) (at level 60, i ident, min at level 60,
 max at level 60, body at level 60, right associativity) : monad_scope.
 
-Definition HoareTriple_L {A} (P : S -> Prop) (m : LoopT A) (B : A -> S -> Prop) : Prop :=
-  forall (s : S), P s -> fun a let (a, s') := m in Q a s'.
+(* Definition LoopT a : Type := (forall (r : Type), (a -> State r) -> State r). *)
+
+(* Definition hoareTripleS {A} (P : S -> Prop) (m : State A) (Q : A -> S -> Prop) : Prop :=
+  forall (s : S), P s -> let (a, s') := m s in Q a s'. *)
+
+(* Au dessus de ma fonction foreach *)
+
+(* Definition HoareTriple_L {A B} (P : Assertion) (m : LoopT A) (Q : B -> Assertion) : Prop :=
+  forall (s : S) (next : A -> State B), P s -> let m' := (runLoopT m next) in let (b,s') := m' s in Q b s'. *)
+
+(* Notation "{{ P }} m {{ Q }}" := (hoareTripleS P m Q)
+  (at level 90, format "'[' '[' {{  P  }}  ']' '/  ' '[' m ']' '['  {{  Q  }} ']' ']'") : monad_scope. *)
+
+Lemma foreach_rule
+  := forall (it:nat) (s : S), (Nat.le min it) /\ (it < max) -> 
+  stepLoopT (body it) (fun _s -> fun a let (a, s') := m 
+  in Q a s'.
 
 End monads.
 
@@ -164,5 +205,5 @@ Definition init_S1 : nat := init_val1.
 fun (S : Type) (f : S -> S) => getS (S:=S) >>= putS (S:=S) ∘ f
      : forall S : Type, (S -> S) -> State S () *)
 
-Definition add_s (i : nat) : State nat unit :=
+Definition add_s (i : nat) : State nat () :=
   modify (fun s => s + i).
